Try to prove some basic results about ingredients and components

Message_Algebra.v
@@ -90,8 +90,14 @@ Inductive key :=
 | Pubk : name -> key
 | Privk : name -> key .
 
+Variable eq_rawkey_dec : forall (x y:rawkey), {x=y} + {x<>y}.
+Hint Resolve eq_rawkey_dec.
 
-Print key_ind.
+Definition eq_key_dec : forall (x y:key), {x=y} + {x<>y}.
+Proof.
+decide equality.
+Qed.
+Hint Resolve eq_key_dec.
 
 Definition invk : key -> key  :=
   fun (k:key) =>
@@ -105,21 +111,68 @@ Definition invk : key -> key  :=
 (** * Main message definitions *)
 
 Inductive msg :=
-| V :  var  -> msg
-| N:  name -> msg
-| D:  data -> msg
+| D : data -> msg
 | K : key -> msg
 | P : msg -> msg -> msg
-| E :  msg -> key -> msg.
+| E : msg -> key -> msg.
 Hint Constructors msg.
 
-(** Treat basic as a predicate, not a subtype *)
+Definition eq_msg_dec : forall x y : msg,  
+  {x = y} + {x <> y}.
+Proof.
+intros.
+decide equality. Qed.
 
+Hint Resolve eq_msg_dec.
+
+(** Atomic values *)
+Inductive is_atomic : msg -> Prop := 
+  |atom : forall x, is_atomic (D x).
+Hint Constructors is_atomic.
+
+(** Concatenated terms or messages *)
+Inductive concat : (msg -> Prop) := 
+  | conc : forall m1 m2, concat (P m1 m2).
+Hint Constructors concat.
+
+(** Encryption *)
+Inductive is_enc : msg -> Prop :=
+  | encr : forall m k, is_enc (E m k).
+Hint Constructors is_enc.
+
+
+(** Treat basic as a predicate, not a subtype *)
 Inductive is_basic : msg -> Prop :=
-| bvar : forall x,  is_basic (V x)
 | bdata : forall x, is_basic (D x)
 | bkey : forall x, is_basic (K x)  .
 Hint Constructors is_basic.
+
+(* Some basic results about atomic and concat *)
+Lemma concat_not_atomic :
+  forall m, concat m -> ~ is_atomic m.
+Proof.
+intros.
+unfold not.
+intros. inversion H. inversion H0.
+symmetry in H1. rewrite H1 in H2.
+discriminate.
+Qed.
+
+Lemma atomic_not_concat:
+  forall m, is_atomic m -> ~concat m.
+Proof.
+intros.
+unfold not. intros.
+inversion H. inversion H0. 
+symmetry in H1. rewrite H1 in H2.
+discriminate.
+Qed.
+
+Lemma enc_not_basic : forall m1 m2, ~ is_basic (P m1 m2).
+Proof.
+intros.
+unfold not. intros. inversion H.
+Qed.
 
 (**  * Three notions of subterm *)
 
@@ -135,7 +188,7 @@ Hint Constructors ingred_1.
 (** *** Transitive closure *)
 Inductive ingred_p (x: msg) : msg -> Prop :=
 | ingred_p_step y  : ingred_1 x y -> ingred_p x y
-| ingred_p_trans y y' : ingred_p x y' -> ingred_p y' y -> ingred_p x y.
+| ingred_p_trans y y' : ingred_1 x y' -> ingred_p y' y -> ingred_p x y.
 Hint Constructors ingred_p.
 
 (** ***  Reflexive-Transitive closure *)
@@ -144,6 +197,32 @@ Inductive ingred (x: msg) : msg -> Prop :=
 | ingred_step y  : ingred_p x y -> ingred x y.
 Hint Constructors ingred.
 
+Lemma ingred_p_transitive : 
+  forall (x y z:msg), ingred_p x y -> ingred_p y z -> ingred_p x z.
+Proof.
+intros.
+induction H.
+apply ingred_p_trans with (y':=y); assumption.
+apply ingred_p_trans with (y':= y'). auto.
+apply IHingred_p. auto.
+Qed.
+
+Lemma ingred_trans : 
+  forall (x y z:msg), ingred x y -> ingred y z -> ingred x z.
+Proof.
+intros.
+induction H; auto.
+inversion H0. subst. 
+apply ingred_step; assumption.
+apply ingred_step.
+apply ingred_p_transitive with (y:=y); assumption.
+Qed.
+
+Lemma ingred_dec : forall x y, {ingred x y} + {~ingred x y}.
+Proof.
+Admitted.
+Hint Resolve ingred_dec.
+Print ingred_ind.
 
 (** ** "Strong ingredient", written as [<<] in EPPSG *)
 (** *** Basis *)
@@ -153,8 +232,8 @@ Inductive strong_ingred_1 :  msg -> msg -> Prop :=
 | strpair2 : forall x y, strong_ingred_1  y (P x y)
 | strenc1  : forall x k, strong_ingred_1 x (E x k)
 | strkeysk :  forall x, strong_ingred_1 (K (Sk x)) (K (Sk x))
-| strkeypubk :  forall n, strong_ingred_1 (N n) (K (Pubk n))
-| strkeyprivk :  forall n, strong_ingred_1 (N n) (K (Privk n))  .
+(*| strkeypubk :  forall n, strong_ingred_1 (N n) (K (Pubk n))
+| strkeyprivk :  forall n, strong_ingred_1 (N n) (K (Privk n))*).
 
 (** ** Transitive  closures *)
 Inductive strong_ingred_p (x: msg) : msg -> Prop :=
@@ -176,8 +255,8 @@ Inductive occurs_in_1 :  msg -> msg -> Prop :=
 | opair2 : forall x y, occurs_in_1  y (P x y)
 | oenc1  : forall x k, occurs_in_1 x (E x k)
 | okeysk :  forall x, occurs_in_1 (K (Sk x)) (K (Sk x))
-| okeypubk :  forall n, occurs_in_1 (N n) (K (Pubk n))
-| okeyprivk :  forall n, occurs_in_1 (N n) (K (Privk n))
+(*| okeypubk :  forall n, occurs_in_1 (N n) (K (Pubk n))
+| okeyprivk :  forall n, occurs_in_1 (N n) (K (Privk n))*)
 | oenc2  : forall x k, occurs_in_1 (K k) (E x k)  .
 
 (** ***  Transitive closure *)
@@ -189,3 +268,37 @@ Inductive occurs_in_p (x: msg) : msg -> Prop :=
 Inductive occurs_in (x: msg) : msg -> Prop :=
 | occurs_in_refl : occurs_in x x
 | occurs_in_step y : occurs_in_p x y -> occurs_in x y.
+
+
+(* existence of maximal encryption
+
+Inductive maximal_enc : msg -> msg -> Prop :=
+  | max_enc1 : forall m1 m2, (ingred m1 m2 /\ is_enc m1 /\ 
+               (forall m, ingred m m2 /\ is_enc m -> ingred m m1)) ->
+               maximal_enc m1 m2.
+
+Lemma exists_1_max_enc : forall m, (exists e, ingred_1 e m /\ is_enc e) -> 
+                          (exists e', maximal_enc e' m).
+Proof.
+intros.
+destruct H as (e, (H1, H2)).
+induction H1.
+exists x. apply max_enc1.
+
+Lemma exists_p_max_enc : forall m, (exists e, ingred_p e m /\ is_enc e) -> 
+                          (exists e', maximal_enc e' m).
+Proof.
+intros.
+destruct H as (e, (H1, H2)).
+induction H1.
+
+Lemma exists_max_enc : forall m, (exists e, ingred e m /\ is_enc e) -> 
+                          (exists e', maximal_enc e' m).
+Proof.
+intros. destruct H as (e, (H1, H2)).
+induction H1. exists e. apply max_enc1.
+repeat split. apply ingred_refl. auto. 
+intros. apply H.
+*)
+
+
